snap

experiments/state_on_io/DMFree.fst
@@ -4,26 +4,29 @@ open FStar.Classical.Sugar
 open FStar.List.Tot.Base
 open FStar.Tactics
 
-open Free
-open Hist
+include Free
+include Hist
 
 (** cmd_wp maps each command to a hist-based WP over events.
     - cmd: command type (parameterizes the free monad)
     - event: event type (parameterizes the hist monad) *)
 let cmd_wp (cmd:Type0 -> Type) (event:Type) = caller -> #r:Type0 -> cmd r -> hist #event r
 
-let guard_wp (#event:Type) (pre:pure_pre) : hist #event (squash pre) =
-  let wp' : hist0 #event (squash pre) = fun p h -> pre /\ p [] () in
-  assert (forall (post1 post2:hist_post #event (squash pre)). (hist_post_ord post1 post2 ==> (forall h. wp' post1 h ==> wp' post2 h)));
-  assert (hist_wp_monotonic wp');
-  wp'
+let cmd_wp_sum
+  #cmd1 #cmd2
+  (#event:Type)
+  (cwp1:cmd_wp cmd1 event)
+  (cwp2:cmd_wp cmd2 event)
+  : cmd_wp (cmd_sum cmd1 cmd2) event =
+  fun c op ->
+    match op with
+    | CmdL op1 -> cwp1 c op1
+    | CmdR op2 -> cwp2 c op2
 
 (** Inspired from Kenji Maillard's thesis (2.4.5) **)
 let rec theta #a #cmd (#event:Type) (cwp:cmd_wp cmd event) (m:free cmd a) : Tot (hist #event a) (decreases m) =
   match m with
   | Return x -> hist_return x
-  | Guard pre k ->
-      hist_bind (guard_wp #event pre) (fun r -> theta cwp (k r))
   | Call c op k ->
       hist_bind (cwp c op) (fun ri -> theta cwp (k ri))
 
@@ -92,35 +95,6 @@ let rec lemma_theta_is_lax_morphism_bind #a #b #cmd (#event:Type) (cwp:cmd_wp cm
       == {}
       theta cwp (free_bind m f);
     }
-  | Guard pre k ->
-    calc (hist_ord) {
-      hist_bind (theta cwp m) (fun x -> theta cwp (f x));
-      == {
-        assert (hist_bind (theta cwp (Guard pre k)) (fun x -> theta cwp (f x))
-           == hist_bind (theta cwp m) (fun x -> theta cwp (f x))) by (rewrite_eqs_from_context ())
-      }
-      hist_bind (theta cwp (Guard pre k)) (fun x -> theta cwp (f x));
-      == { _ by (compute ()) } // unfold theta
-      hist_bind (hist_bind (guard_wp #event pre) (fun r -> theta cwp (k r))) (fun x -> theta cwp (f x));
-      `hist_equiv` { lemma_hist_bind_associativity (guard_wp #event pre) (fun r -> theta cwp (k r)) (fun x -> theta cwp (f x)) }
-      hist_bind (guard_wp #event pre) (fun r -> hist_bind (theta cwp (k r)) (fun x -> theta cwp (f x)));
-      `hist_ord` {
-        let rhs1 = fun r -> hist_bind (theta cwp (k r)) (fun x -> theta cwp (f x)) in
-        let rhs2 = fun r -> theta cwp (free_bind (k r) f) in
-        introduce forall (r:squash pre). (rhs1 r) `hist_ord` (rhs2 r) with begin
-          lemma_theta_is_lax_morphism_bind cwp (k r) f
-        end;
-        another_lemma' (guard_wp #event pre) rhs1 rhs2;
-        assert (hist_bind (guard_wp #event pre) rhs1 `hist_ord` hist_bind (guard_wp #event pre) rhs2) by (assumption ())
-      }
-      hist_bind (guard_wp #event pre) (fun r -> theta cwp (free_bind (k r) f));
-      == { _ by (compute ()) } // unfold theta
-      theta cwp (Guard pre (fun r -> free_bind (k r) f));
-      `hist_ord` { _ by (compute ()) } // unfold free_bind
-      theta cwp (free_bind (Guard pre k) f);
-      == {}
-      theta cwp (free_bind m f);
-    }
 
 // The Dijkstra Monad
 type dm (cmd:Type0 -> Type) (event:Type) (cwp:cmd_wp cmd event) (a:Type) (wp:hist #event a) =
@@ -132,7 +106,7 @@ let dm_return #cmd (#event:Type) (cwp:cmd_wp cmd event) #a (x : a) : dm cmd even
 #push-options "--z3rlimit 40"
 let dm_bind
   #cmd (#event:Type) (cwp:cmd_wp cmd event)
-  #a #b
+  (#a:Type u#a) (#b:Type u#b)
   (wp_v : hist #event a)
   (wp_f: a -> hist #event b)
   (v : dm cmd event cwp a wp_v)
@@ -151,29 +125,3 @@ let dm_subcomp #cmd (#event:Type) (cwp:cmd_wp cmd event) #a (wp1 wp2: hist #even
 let dm_if_then_else #cmd (#event:Type) (cwp:cmd_wp cmd event) #a
   (wp1 wp2: hist #event a) (f : dm cmd event cwp a wp1) (g : dm cmd event cwp a wp2) (b : bool) : Type =
   dm cmd event cwp a (hist_if_then_else wp1 wp2 b)
-
-let dm_guard_return
-  #cmd (#event:Type) (cwp:cmd_wp cmd event)
-  (pre:pure_pre) : dm cmd event cwp (squash pre) (guard_wp #event pre) =
-  let m = Guard pre (Return) in
-  assert ((guard_wp #event pre) `hist_ord` theta cwp m);
-  m
-
-(** Note: the subcomp query (query 6 under --split_queries always) is a
-    pre-existing Z3 limitation with higher-order quantifier instantiation
-    for PURE WP semantics; it also fails on the original (pre-refactor) code
-    without --split_queries. We use assume here. **)
-#push-options "--z3rlimit 40"
-let lift_pure_dm #cmd (#event:Type) (cwp:cmd_wp cmd event)
-  #a
-  (w : pure_wp a)
-  (f:(eqtype_as_type unit -> PURE a w)) :
-  dm cmd event cwp a (wp_lift_pure_hist w) =
-  lemma_wp_lift_pure_hist_implies_as_requires #a #event w;
-  FStar.Monotonic.Pure.elim_pure_wp_monotonicity_forall ();
-  let lhs = dm_guard_return cwp (as_requires w) in
-  let rhs = (fun (pre:(squash (as_requires w))) -> dm_return cwp (f pre)) in
-  let m = dm_bind cwp _ _ lhs rhs in
-  assume (theta cwp m ⊑ wp_lift_pure_hist w);
-  m
-#pop-options
